coq-osiris/theories/program_logic/stop_rules.v
@@ -115,23 +115,19 @@ Section ewp_stop.
 
   Lemma ewp_stop_die {B Y} o (k : _ -> micro B Y) E ι Ψ Φ :
     live_thread ι -∗
+    EWP k o @ E <| (ι, Ψ) |> {{ Φ }} -∗
     EWP (Stop CDie o k) @ E <| (ι, Ψ) |> {{ Φ }}.
   Proof.
-    iIntros "Hι".
+    iIntros "Hι Hwp".
     ewp_unfold_head.
     intro_state.
     iPoseProof (live_thread_valid with "Hti Hι") as "%".
+    assert (ι ∈ dom π). { apply elem_of_dom. eexists. eassumption. }
     ewp_mask_intro "Hmod".
 
     construct_wp_nonret. destruct_wp_step.
     iMod (thread_update with "Hti Hι") as "[Hti Hι]".
     ewp_mask_elim. iFrame.
-    ewp_unfold_head.
-    clear dependent π. clear σ'.
-    intro_state. ewp_mask_intro "Hmod".
-    iPoseProof (dead_thread_valid with "Hti Hι") as "%".
-    construct_wp_nonret. destruct_wp_step.
-    rewrite H in H0. discriminate.
   Qed.
 
   (* When forking a thread, we must prove that the forked thread is
@@ -156,6 +152,7 @@ Section ewp_stop.
     iApply (ewp_mono with "Hcall").
     iIntros (o) "_".
     iApply (ewp_stop_die with "Hlive").
+    destruct o; [ iApply ewp_value | iApply ewp_throw ]; done.
   Qed.
 
   Lemma ewp_fork E Ψ v1 v2 Φ :
